Update interface for QUIC

providers/quic/QuicCrypto.fsti
@@ -26,47 +26,86 @@ module U64 = FStar.UInt64
 module U32 = FStar.UInt32
 module U8 = FStar.UInt8
 
+(*
+This file defines the interface for the packet stream encryption
+functionality. It provides functional correctness with respect
+to the spec in Spec.QUIC of single packet encryption, automatic
+management of the packet stream (using a counter for sending packets
+and a reference to the highest packet number successfully decrypted
+sequence number for incoming packets), and cryptographic security
+of the stream of packets.
+*)
+
 #set-options "--z3rlimit 10 --max_fuel 1 --max_ifuel 1"
 
-[@CAbstractStruct]
-val state_s: Type0
-let state = B.pointer state_s
+// Controls erasure of ideal state
+val model: bool
 
-val freeable_s: state_s -> Type0
-let freeable (h:HS.mem) (p:state) =
-  B.freeable p /\ freeable_s (B.deref h p)
-let preserves_freeable (s:state) (h0 h1:HS.mem): Type0 =
-  freeable h0 s ==> freeable h1 s
-
-val footprint_s: state_s -> GTot B.loc
-let footprint (m:HS.mem) (s:state) =
-  B.(loc_union (loc_addr_of_buffer s) (footprint_s (B.deref m s)))
-
-val inv_s: HS.mem -> state_s -> Type0
-let inv (m:HS.mem) (s:state) =
-  B.live m s /\
-  B.(loc_disjoint (loc_addr_of_buffer s) (footprint_s (B.deref m s))) /\
-  inv_s m (B.get m s 0)
-
-val inv_loc_in_footprint (s:state) (m:HS.mem)
-  : Lemma (requires (inv m s))
-  (ensures ((footprint m s) `M.loc_in` m))
-  [SMTPat (inv m s)]
-
-val frame_inv: l:B.loc -> s:state -> m0:HS.mem -> m1:HS.mem ->
-  Lemma (requires inv m0 s /\ B.loc_disjoint l (footprint m0 s) /\ B.modifies l m0 m1)
-  (ensures inv m1 s /\ footprint m0 s == footprint m1 s)
-
-// Erased to unit when model is off
+// Crypto index, erased to unit when model is off
 val id: eqtype
-val safe: id -> Type
-val is_safe: i:id ->
-  ST bool
+
+// Controls the idealization, false when model is off
+// Internally, safe is defined as honest /\ ideal
+// we assume that honesty is implicit in this interface
+// (i.e. we idealize everything that can be)
+val safe: id -> t:Type{t ==> model}
+val is_safe: i:id -> ST bool
   (requires fun h0 -> True)
   (ensures fun h0 b h1 -> h0 == h1 /\ (b <==> safe i))
 
-val hash_of_id: id -> GTot SQ.ha
-val aead_of_id: id -> GTot SQ.ea
+val defined: id -> Type
+val fresh: id -> mem -> Type
+val is_fresh: i:id -> ST bool
+  (requires fun h0 -> True)
+  (ensures fun h0 b h1 -> if b then defined i else fresh i h1)
+
+// Location for the shared, global ideal state
+val global_loc: M.loc
+
+// State of the packet encryption stream functionality
+[@CAbstractStruct]
+val state_s: id -> Type0
+let state (i:id) = B.pointer (state_s i)
+
+val freeable_s: #i:id -> state_s i -> Type0
+let freeable (#i:id) (h:HS.mem) (p:state i) =
+  B.freeable p /\ freeable_s (B.deref h p)
+let preserves_freeable (#i:id) (s:state i) (h0 h1:HS.mem): Type0 =
+  freeable h0 s ==> freeable h1 s
+
+// Local footprint of an instance, excludes shared global state
+val footprint_s: #i:id -> state_s i -> GTot B.loc
+let footprint (#i:id) (s:state i) (m:HS.mem) =
+  B.(loc_union (loc_addr_of_buffer s) (footprint_s (B.deref m s)))
+
+val inv_s: #i:id -> state_s i -> HS.mem -> Type0
+let inv (#i:id) (s:state i) (m:HS.mem) =
+  B.live m s /\
+  B.(loc_disjoint (loc_addr_of_buffer s) (footprint_s (B.deref m s))) /\
+  inv_s (B.get m s 0) m
+
+val inv_loc_in_footprint (#i:id) (s:state i) (m:HS.mem)
+  : Lemma (requires (inv s m))
+  (ensures ((footprint s m) `M.loc_in` m))
+  [SMTPat (inv s m)]
+
+val frame_inv: #i:id -> s:state i -> m0:HS.mem -> l:B.loc -> m1:HS.mem ->
+  Lemma (requires inv s m0 /\ B.loc_disjoint l (footprint s m0) /\ B.modifies l m0 m1)
+  (ensures inv s m1 /\ footprint s m0 == footprint s m1)
+
+// Ghost access to the index algorithms (when model is on)
+val hash_of_id: id -> Ghost SQ.ha (requires model) (ensures fun _ -> True)
+val aead_of_id: id -> Ghost SQ.ea (requires model) (ensures fun _ -> True)
+
+// Concrete partof the index (agility parameters)
+noeq type info = {
+  region: rid;
+  ha: SQ.ha;
+  ea: SQ.ea;
+}
+
+// Additionaly, the concrete info must be consistent with crypto index
+type info0 (i:id) = a:info{model ==> (hash_of_id i == a.ha /\ aead_of_id i == a.ea)}
 
 type role =
 | Client
@@ -76,22 +115,6 @@ type rw =
 | Writer
 | Reader
 
-// pn s Writer returns the current writing packet number
-// pn s Reader returns the highest packet number successfully decrypted
-val pnT: state_s -> rw -> mem -> GTot nat
-val pn: s:state -> rw:rw -> ST nat
-  (requires fun h0 ->  B.live h0 s /\ inv h0 s)
-  (ensures fun h0 ctr h1 -> h0 == h1 /\
-    ctr == pnT (B.deref h0 s) rw h1)
-
-noeq type info = {
-  region: rid;
-  ha: SHD.hash_alg;
-  ea: SAEAD.alg;
-}
-
-type info0 (i:id) = a:info{hash_of_id i == a.ha /\ aead_of_id i == a.ea}
-
 // Mchine integer version of the QUIC header types
 type u1 = n:U8.t{n = 0z \/ n = 1z}
 type u2 = n:U8.t{U8.v n < 4}
@@ -100,6 +123,27 @@ type u62 = n:UInt64.t{UInt64.v n < pow2 62}
 let add3 (k:u4) : n:U8.t{U8.v n <= 18} = if k = 0uy then 0uy else U8.(k +^ 3uy)
 type vlsize = n:U8.t{U8.v n == 1 \/ U8.v n == 2 \/ U8.v n == 4 \/ U8.v n == 8}
 
+// New streams use the same packet number space in QUIC,
+// we record the initial packet number of the stream and
+// use it as an offset in the packet stream
+val initial_pn: #i:id -> state i -> mem -> GTot SQ.nat62
+val lemma_initial_pn_constant:
+  #i:id -> s:state i -> h0:mem -> h1: mem -> Lemma
+  (requires inv s h0 /\ inv s h1)
+  (ensures initial_pn s h0 == initial_pn s h1)
+
+// pn s Writer returns the current writing packet number
+// pn s Reader returns the highest packet number successfully decrypted
+val pnT: #i:id -> s:state i -> rw -> h:mem -> Ghost SQ.nat62 (requires True)
+  (ensures fun pn -> pn >= initial_pn s h)
+val pn: #i:id -> s:state i -> rw:rw -> ST u62
+  (requires fun h0 ->  B.live h0 s /\ inv s h0)
+  (ensures fun h0 ctr h1 -> h0 == h1 /\ U64.v ctr == pnT s rw h1)
+
+let incrementable (#i:id) (s:state i) (h:mem) =
+  pnT s Writer h + 1 < pow2 62
+
+// Information stored in a QUIC header
 noeq type header =
   | Short:
     spin: u1 ->
@@ -117,6 +161,11 @@ noeq type header =
     plain_len: U32.t{U32.v plain_len < SQ.max_cipher_length} ->
     header
 
+let live_header (h:header) (m:mem) =
+  match h with
+  | Short _ _ _ cid -> m `B.live` cid
+  | Long _ _ _ _ dcid scid _ -> m `B.live` dcid /\ m `B.live` scid
+
 // Converts a concrete header into a spec equivalent
 let spec_header (h:header) (m:HS.mem) : GTot SQ.header =
   match h with
@@ -127,27 +176,50 @@ let spec_header (h:header) (m:HS.mem) : GTot SQ.header =
     (B.as_seq m dcid) (B.as_seq m scid) (U32.v plain_len)
 
 // Packets as recorded by the sender in the ideal log
-type entry =
+type entry (i:id) =
 | Packet:
   pn_len: SQ.nat2 ->
-  h: SQ.header ->
-  p: SQ.pbytes ->
-  entry
+  header: SQ.header ->
+  plain: SQ.pbytes ->
+  packet: SQ.packet ->
+  entry i
+
+// Idealization relies on a global table of ideal state
+// (included in the footprint of every instance)
+val itable: i:id -> h:mem -> GTot (S.seq (entry i))
+
+// Part of the invariant, the size of the log at index i
+// is related to the counter state of any instance at index i
+val lemma_itable_length:
+  #i:id ->
+  s:state i->
+  h:mem -> Lemma
+  (requires inv s h)
+  (ensures S.length (itable i h) == pnT s Writer h - initial_pn s h)
+
+val lemma_itable_frame: i:id -> h0:mem -> l:M.loc -> h1:mem ->
+  Lemma (requires M.modifies l h0 h1 /\ M.loc_disjoint l global_loc)
+  (ensures itable i h0 == itable i h1)
+let modifies_itable (i:id) (h0:mem) (h1:mem) =
+  (forall (j:id{i <> j}). itable j h0 == itable j h1)
 
 (*
 Create a new packet encryption instance from a TLS traffic secret.
 This will perform all the key derivations for the client and server key.
-
 Note that QUIC will create 3 separate instances for the 0-RTT key,
 the handshake encryption key, and the 1-RTT data key.
 *)
 val coerce:
   i: id -> // Erased
   a: info0 i ->
-  dst: B.pointer (B.pointer_or_null state_s) ->
+  initial_pn: u62 ->
+  dst: B.pointer (B.pointer_or_null (state_s i)) ->
   secret: B.buffer U8.t {B.length secret = SHD.hash_length a.ha} ->
   ST error_code
-    (requires fun h0 -> is_eternal_region a.region /\
+    (requires fun h0 -> ~(safe i) /\
+      B.g_is_null (B.deref h0 dst) /\
+      is_eternal_region a.region /\
+      SQ.keysized a.ha (B.length secret) /\
       B.live h0 dst /\ B.live h0 secret)
     (ensures fun h0 e h1 ->
       match e with
@@ -155,62 +227,157 @@ val coerce:
         let s = B.deref h1 dst in
 	SQ.supported_hash a.ha /\
         not (B.g_is_null s) /\
-	inv h1 s /\
+	inv s h1 /\
         M.modifies (M.loc_buffer dst) h0 h1 /\
-        M.fresh_loc (footprint h1 s) h0 h1 /\
-        M.loc_region_only true a.region `M.loc_includes` footprint h1 s /\
-	pnT (B.deref h1 s) Reader h1 == 0 /\
-	pnT (B.deref h1 s) Writer h1 == 0 /\
+        M.fresh_loc (footprint s h1) h0 h1 /\
+        M.loc_region_only true a.region `M.loc_includes` footprint s h1 /\
+	pnT s Reader h1 == U64.v initial_pn /\
+	pnT s Writer h1 == U64.v initial_pn /\
         freeable h1 s
       | _ -> M.modifies M.loc_none h0 h1)
 
-type long_packet_type =
-  | Initial
-  | EarlyData
-  | Handshke
-  | Retry
+val create:
+  i: id -> // Erased
+  a: info0 i ->
+  initial_pn: u62 ->
+  dst: B.pointer (B.pointer_or_null (state_s i)) ->
+  ST error_code
+    (requires fun h0 -> safe i /\
+      B.g_is_null (B.deref h0 dst) /\
+      is_eternal_region a.region /\
+      B.live h0 dst)
+    (ensures fun h0 e h1 ->
+      match e with
+      | Success ->
+        let s = B.deref h1 dst in
+	SQ.supported_hash a.ha /\
+        not (B.g_is_null s) /\
+	inv s h1 /\
+        M.modifies (M.loc_buffer dst) h0 h1 /\
+        M.fresh_loc (footprint s h1) h0 h1 /\
+        M.loc_region_only true a.region `M.loc_includes` footprint s h1 /\
+	pnT s Reader h1 == U64.v initial_pn /\
+	pnT s Writer h1 == U64.v initial_pn /\
+	itable i h1 == S.empty /\
+        freeable h1 s
+      | _ -> M.modifies M.loc_none h0 h1)
 
+val infoT: #i:id -> s:state i -> h:mem -> GTot (info0 i)
+val get_info: #i:id -> s:state i -> ST (info0 i)
+  (requires fun h0 -> inv s h0) (ensures fun h0 a h1 -> h0 == h1 /\ a == infoT s h0)
 
-noeq type header =
-  | Short:
-    spin: U8.t ->
-    phase: U8.t ->
-    cid: B.buffer U8.t{
-      let l = B.length cid in
-      l == 0 \/ (4 <= l /\ l <= 18)} ->
-    header
-  | Long:
-    typ: long_packet_type ->
-    version: U32.t ->
-    dcil: U8.t{U8.v dcil < pow2 4} ->
-    scil: U8.t{U8.v scil < pow2 4} ->
-    dcid: B.buffer U8.t{B.length dcid = SQ.add3 (U8.v dcil)} ->
-    scid: B.buffer U8.t{B.length scid = SQ.add3 (U8.v scil)} ->
-    plain_len: U32.t{U32.v plain_len <= SQ.max_plain_length} ->
-    header
+val leakT: #i:id -> s:state i -> h:mem ->
+  Ghost (SQ.lbytes (SHD.hash_length (infoT s h).ha)) 
+  (requires inv s h /\ ~(safe i))
+  (ensures fun b -> SQ.keysized (infoT s h).ha (S.length b))
 
-let spec_header (h:header) (m:mem) : GTot SQ.header =
-  match h with
-  | Short spin phase cid ->
-    SQ.Short
-      (spin=1z)
-      (phase=1z)
-      (LowStar.Buffer.as_seq m cid)
-  | Long typ version dcil scil dcid scid len ->
-    admit()
+let if_safe (i:id) (t:Type) (f:Type) =
+  (safe i ==> t) /\ (~(safe i) ==> f)
 
-//val writer_log: s:state -> h:HS.mem -> GTot (S.seq (S.seq SQ.bytes))
-
-(*
+(* QUIC HKDF labels, move to Spec.QUIC? *)
+val label_key : SQ.lbytes 3
+val label_iv : SQ.lbytes 2
+val label_hp : SQ.lbytes 2
 
 val encrypt:
-  st: state ->
-  
-  
+  #i:id -> // Erased
+  s: state i ->
+  h: header ->
+  plain_len: U32.t{3 <= U32.v plain_len /\ U32.v plain_len < SQ.max_plain_length} ->
+  plain: B.lbuffer U8.t (U32.v plain_len) ->
+  pn_len: u2 ->
+  out: B.buffer U8.t ->
+  ST error_code
+  (requires fun h0 -> B.live h0 plain /\ B.live h0 out /\
+    inv s h0 /\ live_header h h0 /\ incrementable s h0 /\
+    (let clen = U32.v plain_len + SAEAD.tag_length (infoT s h0).ea in
+    let len = clen + SQ.header_len (spec_header h h0) (U8.v pn_len) in
+    (Long? h ==> U32.v (Long?.plain_len h) = clen) /\
+    B.length out == len))
+  (ensures fun h0 r h1 ->
+    let fp = M.loc_union (M.loc_buffer out)
+      (M.loc_union global_loc (footprint s h0)) in
+    M.modifies fp h0 h1 /\
+    modifies_itable i h0 h1 /\
+    (match r with
+    | Success ->
+      inv s h1 /\
+      pnT s Writer h1 == pnT s Writer h0 + 1 /\
+      (safe i ==>
+       begin (* Ideal case *)
+        let log0 = itable i h0 in
+	let log1 = itable i h1 in
+	log1 == S.append log0
+	  (S.create 1 (Packet (U8.v pn_len) (spec_header h h0)
+	    (B.as_seq h0 plain) (B.as_seq h1 out)))
+       end) /\
+      ~(safe i) ==>
+       begin (* Concrete case *)
+        let a = infoT s h0 in
+        let s0 = leakT s h0 in
+        let k = SQ.derive_secret a.ha s0 label_key (SAEAD.key_length a.ea) in
+        let iv = SQ.derive_secret a.ha s0 label_iv 12 in
+        let pne = SQ.derive_secret a.ha s0 label_hp (SQ.ae_keysize a.ea) in
+	let plain : SQ.pbytes = B.as_seq h0 plain in
+	let packet : SQ.packet = B.as_seq h1 out in
+	let ctr = pnT s Writer h0 in
+	packet == SQ.encrypt a.ea k iv pne (U8.v pn_len) ctr (spec_header h h0) plain
+       end
+    | _ -> True))
+
+noeq type result = {
+  pn_len: u2;
+  pn: u62;
+  plain_len: n:U32.t{let l = U32.v n in 3 <= l /\ l < SQ.max_plain_length};
+  plain: B.buffer U8.t;
+}
 
 val decrypt:
+  #i:id -> // Erased
+  s: state i ->
+  len: U32.t{21 <= U32.v len /\ U32.v len < pow2 32} ->
+  packet: B.lbuffer U8.t (U32.v len) ->
+  cid_len: u4 ->
+  header: B.pointer header ->
+  out: B.pointer result ->
+  ST error_code
+  (requires fun h0 -> B.live h0 packet /\ B.live h0 header /\ B.live h0 out /\
+    inv s h0 /\ (Long? (B.deref h0 header) ==> cid_len = 0z))
+  (ensures fun h0 r h1 ->
+    M.modifies (M.loc_union (footprint s h0)
+      (M.loc_buffer header `M.loc_union` M.loc_buffer out)) h0 h1 /\
+    (match r with
+    | Success ->
+      let o = B.deref h1 out in
+      let h = B.deref h1 header in
+      let pn = U64.v o.pn in
+      let last = pnT s Reader h0 in
+      inv s h1 /\ pn >= initial_pn s h0 /\
+      pnT s Reader h1 == U64.v o.pn /\
+      B.length o.plain == U32.v o.plain_len /\
+      (safe i ==>
+       begin (* Ideal case *)
+        let log0 = itable i h0 in
+	let log1 = itable i h1 in
+	log0 == log1 /\
+	pn - initial_pn s h0 < S.length log0 /\
+	S.index log0 (pn - initial_pn s h0) ==
+	  (Packet (U8.v o.pn_len) (spec_header h h1)
+	    (B.as_seq h0 o.plain) (B.as_seq h0 packet))
+       end) /\
+      ~(safe i) ==>
+       begin (* Concrete case *)
+        let a = infoT s h0 in
+        let s0 = leakT s h0 in
 
-val rekey:
+        let k = SQ.derive_secret a.ha s0 label_key (SAEAD.key_length a.ea) in
+        let iv = SQ.derive_secret a.ha s0 label_iv 12 in
+        let pne = SQ.derive_secret a.ha s0 label_hp (SQ.ae_keysize a.ea) in
+	let plain : SQ.pbytes = B.as_seq h0 o.plain in
+	let packet : SQ.packet = B.as_seq h0 packet in
+	let last = pnT s Reader h0 in
+	SQ.decrypt a.ea k iv pne last (U8.v cid_len) packet
+	  == SQ.Success (U8.v o.pn_len) (U64.v o.pn) (spec_header h h1) plain
+       end
+    | _ -> True))
 
-val free:
-*)
